HarderNarasimhan/Filtration/Results.lean
@@ -59,4 +59,334 @@ where
     exact fun j hij hj ↦ this j hij hj
   ) n)
 
+
+theorem exists_relSeries_isIntervalSemistable {ℒ : Type*} [Nontrivial ℒ] [Lattice ℒ] [BoundedOrder ℒ] [WellFoundedGT ℒ]
+{S : Type*} [CompleteLattice S]
+(μ : {p :ℒ × ℒ // p.1 < p.2} → S)
+[hμ : μA_DescendingChainCondition μ] [hμcvx : Convex μ] [h : μ_Admissible μ] :
+------------
+∃ s : RelSeries (IsIntervalSemistable μ),
+  s.head = ⊥ ∧ s.last = ⊤ ∧
+  ∀ i : ℕ, (hi : i + 1 < s.length) →
+    ¬   μA μ ⟨(s.toFun i, s.toFun ↑(i+1)), by simp [*]⟩
+      ≤ μA μ ⟨(s.toFun ↑(i+1), s.toFun ↑(i+2)), by simp [*]⟩
+------------
+ := by
+  let HNfil : HarderNarasimhanFiltration μ := default
+  let HNseq : RelSeries (IsIntervalSemistable μ) := {
+    toFun := fun n ↦ HNfil.filtration n,
+    length := Nat.find HNfil.fin_len
+    step := by
+      intro i
+      use HNfil.strict_mono i.val (i.succ).val (Nat.lt_add_one i.val) <| Fin.is_le i.succ
+      exact HNfil.piecewise_semistable i.val i.prop
+  }
+  use HNseq
+  refine ⟨rfl,Nat.find_spec HNfil.fin_len,?_⟩
+  refine fun i hi hc ↦ HNfil.μA_pseudo_strict_anti i hi ?_
+  convert hc
+  · simp only [Fin.val_natCast]
+    refine Eq.symm (Nat.mod_eq_of_lt ?_)
+    exact lt_trans (Nat.lt_add_one i) <| lt_trans hi (Nat.lt_add_one _)
+  · simp only [Fin.val_natCast]
+    refine Eq.symm (Nat.mod_eq_of_lt ?_)
+    exact lt_trans hi (Nat.lt_add_one _)
+  · simp only [Fin.val_natCast]
+    refine Eq.symm (Nat.mod_eq_of_lt ?_)
+    exact lt_trans hi (Nat.lt_add_one _)
+  · simp only [Fin.val_natCast]
+    refine Eq.symm (Nat.mod_eq_of_lt ?_)
+    exact Nat.succ_lt_succ hi
+
+theorem exists_unique_relSeries_isIntervalSemistable_of_completeLinearOrder {ℒ : Type*} [Nontrivial ℒ] [Lattice ℒ] [BoundedOrder ℒ] [WellFoundedGT ℒ]
+{S : Type*} [CompleteLinearOrder S]
+(μ : {p :ℒ × ℒ // p.1 < p.2} → S)
+[hμ : μA_DescendingChainCondition μ] [hμcvx : Convex μ]:
+------------
+∃! s : RelSeries (IsIntervalSemistable μ),
+  s.head = ⊥ ∧ s.last = ⊤ ∧
+  ∀ i : ℕ, (hi : i + 1 < s.length) →
+    ¬   μA μ ⟨(s.toFun i, s.toFun ↑(i+1)), by simp [*]⟩
+      ≤ μA μ ⟨(s.toFun ↑(i+1), s.toFun ↑(i+2)), by simp [*]⟩
+------------
+:= by
+  apply existsUnique_of_exists_of_unique
+  · exact exists_relSeries_isIntervalSemistable μ
+  · intro F1 F2 h1 h2
+    let filtration1 := fun n ↦ if n ≤ F1.length then F1.toFun n else ⊤
+    have hstrange : ∃ n, (if n ≤ F1.length then F1.toFun ↑n else ⊤) = ⊤ := by
+      use F1.length
+      simp only [le_refl, Fin.natCast_eq_last]
+      exact h1.2.1
+    have hslen : Nat.find hstrange  = F1.length := by
+      have := Nat.find_min' hstrange ((by
+        unfold filtration1
+        simp only [le_refl, ↓reduceIte, Fin.natCast_eq_last, filtration1]
+        exact h1.2.1
+        ) : filtration1 F1.length = ⊤)
+      refine le_antisymm this ?_
+      by_contra hc
+      apply lt_of_not_le at hc
+      have t := Nat.find_spec hstrange
+      simp only [if_pos this] at t
+
+      sorry
+    let HN1 : HarderNarasimhanFiltration μ := {
+      filtration := filtration1,
+      monotone := by
+        refine monotone_nat_of_le_succ ?_
+        intro n
+        if hn : n ≤ F1.length then
+          simp only [filtration1,hn, ↓reduceIte]
+          if hn' : n + 1 ≤ F1.length then
+            simp only [hn', ↓reduceIte]
+            have := le_of_lt (F1.step ⟨n,hn'⟩).choose
+            convert this
+            · simp only [Fin.castSucc_mk]
+              refine Fin.eq_mk_iff_val_eq.mpr ?_
+              refine Fin.val_cast_of_lt ?_
+              exact Nat.lt_add_right 1 hn'
+            · simp
+              refine Fin.eq_mk_iff_val_eq.mpr ?_
+              refine Fin.val_cast_of_lt ?_
+              exact Nat.add_lt_add_right hn' 1
+          else
+          simp only [hn', ↓reduceIte, le_top]
+        else
+        simp only [filtration1,hn, ↓reduceIte, top_le_iff, ite_eq_right_iff]
+        intro hn'
+        exfalso
+        linarith
+        ,
+      first_eq_bot := by
+        simp only [filtration1,zero_le, ↓reduceIte]
+        exact h1.1
+        ,
+      fin_len := by
+        use F1.length
+        simp only [filtration1,le_refl, ↓reduceIte, Fin.natCast_eq_last]
+        exact h1.2.1
+        ,
+      strict_mono := by
+        intro i j hij hj
+        rw [hslen] at hj
+        simp [hj,le_of_lt <| lt_of_lt_of_le hij hj,filtration1]
+        sorry,
+      piecewise_semistable := by
+        intro i hi
+        have := (F1.step ⟨i,hslen ▸ hi⟩).choose_spec
+        unfold filtration1
+        simp
+        rw [hslen] at hi
+        convert this
+        · simp [le_of_lt hi]
+          congr
+          refine Fin.eq_mk_iff_val_eq.mpr ?_
+          refine Fin.val_cast_of_lt ?_
+          exact Nat.lt_add_right 1 hi
+        · have this': i + 1 ≤ F1.length := by linarith
+          simp [this']
+          congr
+          refine Fin.eq_mk_iff_val_eq.mpr ?_
+          refine Fin.val_cast_of_lt ?_
+          linarith
+        · simp [le_of_lt hi]
+          congr
+          refine Fin.eq_mk_iff_val_eq.mpr ?_
+          refine Fin.val_cast_of_lt ?_
+          exact Nat.lt_add_right 1 hi
+        · have this' : i + 1 ≤ F1.length := by linarith
+          simp [this']
+          congr
+          refine Fin.eq_mk_iff_val_eq.mpr ?_
+          refine Fin.val_cast_of_lt ?_
+          linarith
+        · simp [le_of_lt hi]
+          congr
+          refine Fin.eq_mk_iff_val_eq.mpr ?_
+          refine Fin.val_cast_of_lt ?_
+          exact Nat.lt_add_right 1 hi
+        · have this' : i + 1 ≤ F1.length := by linarith
+          simp [this']
+          congr
+          refine Fin.eq_mk_iff_val_eq.mpr ?_
+          refine Fin.val_cast_of_lt ?_
+          linarith
+        · simp [le_of_lt hi]
+          congr
+          refine Fin.eq_mk_iff_val_eq.mpr ?_
+          refine Fin.val_cast_of_lt ?_
+          exact Nat.lt_add_right 1 hi
+        · have this' : i + 1 ≤ F1.length := by linarith
+          simp [this']
+          congr
+          refine Fin.eq_mk_iff_val_eq.mpr ?_
+          refine Fin.val_cast_of_lt ?_
+          linarith
+        ,
+      μA_pseudo_strict_anti := by
+        intro i hi
+        have := h1.2.2 i (hslen ▸ hi)
+        unfold filtration1
+        rw [hslen] at hi
+        convert this
+        · have this' : i ≤ F1.length := by linarith
+          simp [this']
+        · simp [le_of_lt hi]
+        · simp [le_of_lt hi]
+        · have : i + 2 ≤ F1.length := by omega
+          simp [this]
+    }
+    let filtration2 := fun n ↦ if n ≤ F2.length then F2.toFun n else ⊤
+    have hstrange2 : ∃ n, (if n ≤ F2.length then F2.toFun ↑n else ⊤) = ⊤ := by
+      use F2.length
+      simp
+      exact h2.2.1
+    have hslen : Nat.find hstrange2  = F2.length := by
+      have := Nat.find_min' hstrange2 ((by
+        unfold filtration2
+        simp only [le_refl, ↓reduceIte, Fin.natCast_eq_last, filtration2]
+        exact h2.2.1
+        ) : filtration2 F2.length = ⊤)
+      refine le_antisymm this ?_
+      by_contra hc
+      apply lt_of_not_le at hc
+      have t := Nat.find_spec hstrange
+      simp only [if_pos this] at t
+
+      sorry
+    let HN2 : HarderNarasimhanFiltration μ := {
+      filtration := filtration2,
+      monotone := by
+        refine monotone_nat_of_le_succ ?_
+        intro n
+        if hn : n ≤ F2.length then
+          simp only [filtration2,hn, ↓reduceIte]
+          if hn' : n + 1 ≤ F2.length then
+            simp only [hn', ↓reduceIte]
+            have := le_of_lt (F2.step ⟨n,hn'⟩).choose
+            convert this
+            · simp only [Fin.castSucc_mk]
+              refine Fin.eq_mk_iff_val_eq.mpr ?_
+              refine Fin.val_cast_of_lt ?_
+              exact Nat.lt_add_right 1 hn'
+            · simp
+              refine Fin.eq_mk_iff_val_eq.mpr ?_
+              refine Fin.val_cast_of_lt ?_
+              exact Nat.add_lt_add_right hn' 1
+          else
+          simp only [hn', ↓reduceIte, le_top]
+        else
+        simp only [filtration2,hn, ↓reduceIte, top_le_iff, ite_eq_right_iff]
+        intro hn'
+        exfalso
+        linarith
+        ,
+      first_eq_bot := by
+        simp only [filtration2,zero_le, ↓reduceIte]
+        exact h2.1
+        ,
+      fin_len := by
+        use F2.length
+        simp only [filtration2,le_refl, ↓reduceIte, Fin.natCast_eq_last]
+        exact h2.2.1
+        ,
+      strict_mono := by
+        intro i j hij hj
+        rw [hslen] at hj
+        simp [hj,le_of_lt <| lt_of_lt_of_le hij hj,filtration2]
+        sorry,
+      piecewise_semistable := by
+        intro i hi
+        have := (F2.step ⟨i,hslen ▸ hi⟩).choose_spec
+        unfold filtration2
+        simp
+        rw [hslen] at hi
+        convert this
+        · simp [le_of_lt hi]
+          congr
+          refine Fin.eq_mk_iff_val_eq.mpr ?_
+          refine Fin.val_cast_of_lt ?_
+          exact Nat.lt_add_right 1 hi
+        · have this': i + 1 ≤ F2.length := by linarith
+          simp [this']
+          congr
+          refine Fin.eq_mk_iff_val_eq.mpr ?_
+          refine Fin.val_cast_of_lt ?_
+          linarith
+        · simp [le_of_lt hi]
+          congr
+          refine Fin.eq_mk_iff_val_eq.mpr ?_
+          refine Fin.val_cast_of_lt ?_
+          exact Nat.lt_add_right 1 hi
+        · have this' : i + 1 ≤ F2.length := by linarith
+          simp [this']
+          congr
+          refine Fin.eq_mk_iff_val_eq.mpr ?_
+          refine Fin.val_cast_of_lt ?_
+          linarith
+        · simp [le_of_lt hi]
+          congr
+          refine Fin.eq_mk_iff_val_eq.mpr ?_
+          refine Fin.val_cast_of_lt ?_
+          exact Nat.lt_add_right 1 hi
+        · have this' : i + 1 ≤ F2.length := by linarith
+          simp [this']
+          congr
+          refine Fin.eq_mk_iff_val_eq.mpr ?_
+          refine Fin.val_cast_of_lt ?_
+          linarith
+        · simp [le_of_lt hi]
+          congr
+          refine Fin.eq_mk_iff_val_eq.mpr ?_
+          refine Fin.val_cast_of_lt ?_
+          exact Nat.lt_add_right 1 hi
+        · have this' : i + 1 ≤ F2.length := by linarith
+          simp [this']
+          congr
+          refine Fin.eq_mk_iff_val_eq.mpr ?_
+          refine Fin.val_cast_of_lt ?_
+          linarith
+        ,
+      μA_pseudo_strict_anti := by
+        intro i hi
+        have := h2.2.2 i (hslen ▸ hi)
+        unfold filtration2
+        rw [hslen] at hi
+        convert this
+        · have this' : i ≤ F2.length := by linarith
+          simp [this']
+        · simp [le_of_lt hi]
+        · simp [le_of_lt hi]
+        · have : i + 2 ≤ F2.length := by omega
+          simp [this]
+    }
+    have t1 := instUniqueHarderNarasimhanFiltration.uniq HN1
+    have t2 := instUniqueHarderNarasimhanFiltration.uniq HN2
+    have := t2.symm ▸ t1
+    have len_eq : F1.length = F2.length := by
+      expose_names
+      rw [← hslen_1]
+      have : Nat.find HN1.fin_len = Nat.find HN2.fin_len := by
+        rw [this]
+      rw [this,hslen]
+    ext x
+    · exact len_eq
+    · simp only [Function.comp_apply]
+      have : HN1.filtration x.val = HN2.filtration x.val := by
+        rw [this]
+      have : filtration1 x.val = filtration2 x.val := by
+        exact this
+      unfold filtration1 filtration2 at this
+      simp only [Fin.is_le x, ↓reduceIte, Fin.cast_val_eq_self] at this
+      have t' := Fin.is_le x
+      simp only [len_eq] at t'
+      simp only [t', ↓reduceIte] at this
+      convert this
+      refine Fin.eq_of_val_eq ?_
+      simp only [Fin.coe_cast, Fin.val_natCast]
+      refine Eq.symm (Nat.mod_eq_of_lt ?_)
+      exact Nat.lt_add_one_of_le t'
+
+
 end HarderNarasimhan
